backends/lean/Base/Arith.lean
@@ -1,2 +1,3 @@
 import Base.Arith.Int
 import Base.Arith.Scalar
+import Base.Arith.Lemmas
